coq-osiris/theories/lang/syntax.v
@@ -1,5 +1,5 @@
 From osiris Require Import base.
-From osiris.lang Require Import float int char locations.
+From osiris.lang Require Import float int char locations thread_ids.
 
 (* This file should be in sync with osiris/src/Syntax.ml. *)
 
@@ -412,6 +412,8 @@ Inductive val :=
   | VRecord (fvs : list (var * val))
   (* A location. *)
   | VLoc (l: loc)
+  (* A thread id. *)
+  | VThread (t: thread)
   (* A continuation; more precisely, a location which stores a continuation. *)
   | VCont (k: cont)
   (* A module. *)
